sensitive attrs hiding instantiation with ind_cpa

ID_system_formalisation/IDentity.thy
@@ -7,36 +7,39 @@ sledgehammer_params[timeout = 1000]
 
 type_synonym ('share1', 'share2', 'share3') share_user_record = "'share1' \<times> 'share2' \<times> 'share3'"
 
-type_synonym 'attrs' query = "'attrs' \<Rightarrow> bool"
+type_synonym ('attrs', 'sens_atrrs', 'result') query = "('attrs' set \<times> 'sens_atrrs' set) \<Rightarrow> 'result'"
 
-type_synonym ('attrs', 'state_attr_hid',  'enc_attrs') attr_hiding_adversary = "(('attrs' \<times> 'attrs') \<times> 'state_attr_hid') spmf \<times> ('state_attr_hid' \<Rightarrow> 'enc_attrs' \<Rightarrow> bool spmf)"
+type_synonym ('attrs', 'sens_atrrs') user_attrs = "('attrs' set \<times> 'sens_atrrs' set)" 
+
+type_synonym ('user', 'state_attr_hid', 'enc_attrs') attr_hiding_adversary
+            = "(('user' \<times> 'user') \<times> 'state_attr_hid') spmf \<times> ('state_attr_hid' \<Rightarrow> 'enc_attrs' \<Rightarrow> bool spmf)"
 
 type_synonym ('token', 'state',  'auth_token') hiding_adversary = "(('token' \<times> 'token') \<times> 'state') spmf \<times> ('state' \<Rightarrow> 'auth_token' \<Rightarrow> bool spmf)"
 
 type_synonym 'token' soundness_adversary = "'token' \<Rightarrow> 'token' spmf"
 
-locale identity =
-  fixes reg_user :: "'attrs \<Rightarrow> 'enc_attrs spmf" \<comment> \<open>The user encrypts their attributes before sending them to the government.\<close> 
-    and reg_govt_shares :: "'enc_attrs \<Rightarrow> (('share1, 'share2, 'share3) share_user_record \<times> 'state_govt) spmf"
+locale identity_system =
+  fixes reg_enc_sens_attrs :: "'sens_atrrs set \<Rightarrow> 'enc_attrs spmf" \<comment> \<open>The user encrypts their attributes before sending them to the government.\<close> 
+    and reg_govt_shares :: "'attrs set \<Rightarrow> 'enc_attrs \<Rightarrow> (('share1, 'share2, 'share3) share_user_record \<times> 'state_govt) spmf"
     and reg_govt_token :: "'state_govt \<Rightarrow> ('share1, 'share2, 'share3) share_user_record \<Rightarrow> 'token spmf"
 \<comment> \<open>The government first produces the shares of the user record and then a token to be sent back to the user.\<close>
-    and auth :: "'token \<Rightarrow> 'attrs query \<Rightarrow> 'auth_token spmf" 
+    and auth :: "'token \<Rightarrow> ('attrs, 'sens_atrrs, 'result) query \<Rightarrow> 'auth_token spmf" 
 \<comment> \<open>Authentication is run between a user and a service provider. 
     The user inputs their token, the service provider their desired query and an authorised token is returned. This is sent to the government.\<close>
-    and ver :: "'auth_token \<Rightarrow> bool spmf"
+    and ver :: "'auth_token \<Rightarrow> 'result spmf"
 \<comment> \<open>The government uses the authorised token to determine the response to the query.\<close>
     and valid_user :: "'user \<Rightarrow> bool"
-    and valid_attrs :: "'attrs \<Rightarrow> bool" 
+    and valid_attrs :: "('attrs set \<times> 'sens_atrrs set) \<Rightarrow> bool" 
     and valid_token :: "'token \<Rightarrow> bool"
-    and valid_query :: "'attrs query \<Rightarrow> bool"
+    and valid_query :: "('attrs, 'sens_atrrs, 'result) query \<Rightarrow> bool"
     and user_set :: "'user set"
-    and attrs_set :: "'attrs set"
-    and users_to_attributes :: "'user \<Rightarrow> 'attrs"
+    and attrs_set :: "('attrs set \<times> 'sens_atrrs set) set"
+    and users_attr_creation :: "'user \<Rightarrow> ('attrs set \<times> 'sens_atrrs set)"
   assumes users_are_valid: "user \<in> user_set \<longrightarrow> valid_user user"
     and atrrs_are_valid: "attrs \<in> attrs_set \<longrightarrow> valid_attrs attrs"
     and user_set_not_empty: "user_set \<noteq> {}"
     and attrs_set_not_empty: "attrs_set \<noteq> {}"
-    and bij_betw_users_attrs: "bij_betw users_to_attributes user_set attrs_set"
+    and bij_betw_users_attrs: "bij_betw users_attr_creation user_set attrs_set"
     (*and service_providers :: "'providers set"
     and fed_govt :: "'dept set" *)
 (*user sets can be parameters of the system, what assumptions need to be made on them?*)
@@ -52,9 +55,9 @@ text\<open>We define the registration phase using the fixes parameters for the u
 
 definition reg :: "'user \<Rightarrow> ('token \<times> ('share1, 'share2, 'share3) share_user_record) spmf" 
   where "reg user = do {
-   let attrs = users_to_attributes user;
-   enc_attrs \<leftarrow> reg_user attrs;
-   (S, \<sigma>) \<leftarrow> reg_govt_shares enc_attrs;
+   let (attrs, sens_attrs) = users_attr_creation user;
+   enc_attrs \<leftarrow> reg_enc_sens_attrs sens_attrs;
+   (S, \<sigma>) \<leftarrow> reg_govt_shares attrs enc_attrs;
    token \<leftarrow> reg_govt_token \<sigma> S;
    return_spmf (token, S)}"
 
@@ -63,16 +66,15 @@ subsection\<open>Functional Properties\<close>
 lemma obtain_user_from_attrs:
   fixes attrs
   assumes "attrs \<in> attrs_set"
-  obtains user where "user \<in> user_set" and "users_to_attributes user = attrs"
+  obtains user where "user \<in> user_set" and "users_attr_creation user = attrs"
   using bij_betw_users_attrs[unfolded bij_betw_def] assms
   by auto 
 
 lemma obtain_attrs_from_user:
   fixes user
   assumes "user \<in> user_set"
-  obtains attrs where "attrs \<in> attrs_set" "users_to_attributes user = attrs"
-  using bij_betw_users_attrs[unfolded bij_betw_def] assms
-  by auto 
+  obtains attrs where "attrs \<in> attrs_set" "users_attr_creation user = attrs"
+  using bij_betw_users_attrs[unfolded bij_betw_def] assms by blast
 
 text\<open>We require that that no two users, with different attributes, will yield the same tokens upon registration. This must be a property of the registration phase the attributes.\<close>
 
@@ -80,9 +82,9 @@ definition "unique_users = (\<forall> user1 user2. user1 \<in> user_set \<longri
 
 text \<open>The correctness property ensures if the IDentity system is carried out honestly the correct query result is returned.\<close>
 
-definition correct_game :: "'user \<Rightarrow> 'attrs query \<Rightarrow> bool spmf"
+definition correct_game :: "'user \<Rightarrow> ('attrs, 'sens_atrrs, 'result) query \<Rightarrow> bool spmf"
   where "correct_game user query = do {
-        let attrs = users_to_attributes user;
+        let attrs = users_attr_creation user;
         (token, enc_user_record) \<leftarrow> reg user;
         auth_token \<leftarrow> auth token query;
         b \<leftarrow> ver auth_token;
@@ -90,46 +92,183 @@ definition correct_game :: "'user \<Rightarrow> 'attrs query \<Rightarrow> bool 
 
 definition "correct \<longleftrightarrow> (\<forall> user query. valid_user user \<longrightarrow> valid_query query \<longrightarrow> spmf (correct_game user query) True = 1)"
 
-primrec reg_attrs_hiding_game :: "('attrs, 'state_attr_hid,  'enc_attrs) attr_hiding_adversary \<Rightarrow> bool spmf"
+primrec sens_attrs_hiding_game :: "('user, 'state_attr_hid, 'enc_attrs) attr_hiding_adversary \<Rightarrow> bool spmf"
   where 
-    "reg_attrs_hiding_game (\<A>1, \<A>2) = do {
-      ((attrs0, attrs1), \<sigma>) \<leftarrow> \<A>1;
+    "sens_attrs_hiding_game (\<A>1, \<A>2) = TRY do {
+      ((user0, user1), \<sigma>) \<leftarrow> \<A>1;
+      _ :: unit \<leftarrow> assert_spmf (valid_user user0 \<and> valid_user user1);
       b \<leftarrow> coin_spmf;
-      enc_attrs_b \<leftarrow> reg_user (if b then attrs1 else attrs0);
+      let (attrsb, sens_attrsb) = users_attr_creation (if b then user0 else user1);
+      enc_attrs_b \<leftarrow> reg_enc_sens_attrs sens_attrsb;
       b' \<leftarrow> \<A>2 \<sigma> enc_attrs_b;
-      return_spmf (b = b')}" 
+      return_spmf (b' = b)} ELSE coin_spmf" 
 
-definition "reg_attrs_hiding_advantage \<A> = \<bar>spmf (reg_attrs_hiding_game \<A>) True - 1/2\<bar>"
+definition "sens_attrs_hiding_advantage \<A> = \<bar>spmf (sens_attrs_hiding_game \<A>) True - 1/2\<bar>"
 
-definition "perfect_reg_attrs_hiding \<A> \<longleftrightarrow> reg_attrs_hiding_advantage \<A> = 0"
+definition "perfect_sens_attrs_hiding \<A> \<longleftrightarrow> sens_attrs_hiding_advantage \<A> = 0"
 
-definition hiding_game :: "'attrs query \<Rightarrow> ('token, 'state,  'auth_token) hiding_adversary \<Rightarrow> bool spmf"
-  where "hiding_game query \<A> = do {
-        let (\<A>1, \<A>2) = \<A>;
-        ((token0, token1), \<sigma>) \<leftarrow> \<A>1;
-        _ :: unit \<leftarrow> assert_spmf (valid_token token0 \<and> valid_token token1);
-        b \<leftarrow> coin_spmf;
-        auth_token \<leftarrow> auth (if b then token1 else token0) query;
-        b' \<leftarrow> \<A>2 \<sigma> auth_token;  
-        return_spmf (b = b')}"
+definition "no_sens_attr \<longleftrightarrow> (\<forall> user. snd (users_attr_creation user) = {})"
 
-definition "hiding_advantage query \<A> = (\<bar>spmf (hiding_game query \<A>) True - 1/2\<bar>)"
+lemma 
+  assumes "no_sens_attr"
+  shows "perfect_sens_attrs_hiding \<A>"
+  including monad_normalisation
+proof-
+  note [simp] = Let_def split_def 
+  have "\<bar>spmf (sens_attrs_hiding_game \<A>) True - 1/2\<bar> = 0"
+  proof-
+    obtain \<A>1 and \<A>2 where \<A> [simp]: "\<A> = (\<A>1, \<A>2)" by(cases \<A>)
+    have "sens_attrs_hiding_game (\<A>1, \<A>2) = TRY do {
+      ((user0, user1), \<sigma>) \<leftarrow> \<A>1;
+      _ :: unit \<leftarrow> assert_spmf (valid_user user0 \<and> valid_user user1);
+      b \<leftarrow> coin_spmf;
+      let (attrsb, sens_attrsb) = users_attr_creation (if b then user0 else user1);
+      enc_attrs_b \<leftarrow> reg_enc_sens_attrs sens_attrsb;
+      b' \<leftarrow> \<A>2 \<sigma> enc_attrs_b;
+      return_spmf (b' = b)} ELSE coin_spmf"
+      by(simp add: sens_attrs_hiding_game_def)
+    also have "... = TRY do {
+      ((user0, user1), \<sigma>) \<leftarrow> \<A>1;
+      _ :: unit \<leftarrow> assert_spmf (valid_user user0 \<and> valid_user user1);
+      b :: bool \<leftarrow> coin_spmf;
+      enc_attrs_b \<leftarrow> reg_enc_sens_attrs {};
+      b' :: bool \<leftarrow> \<A>2 \<sigma> enc_attrs_b;
+      return_spmf (b' = b)} ELSE coin_spmf"
+      using assms[unfolded no_sens_attr_def] 
+      by simp
+    also have "... = TRY do {
+      ((user0, user1), \<sigma>) \<leftarrow> \<A>1;
+      _ :: unit \<leftarrow> assert_spmf (valid_user user0 \<and> valid_user user1);
+      enc_attrs_b \<leftarrow> reg_enc_sens_attrs {};
+      b' :: bool \<leftarrow> \<A>2 \<sigma> enc_attrs_b;
+      map_spmf((=) b') coin_spmf} ELSE coin_spmf"
+      by(simp add: map_spmf_conv_bind_spmf)
+    also have "... = coin_spmf" 
+      by(auto simp add: bind_spmf_const map_eq_const_coin_spmf try_bind_spmf_lossless2' scale_bind_spmf weight_spmf_le_1 scale_scale_spmf)
+    ultimately show ?thesis  
+      by(simp add: spmf_of_set)
+  qed
+  thus ?thesis 
+    by(simp add: perfect_sens_attrs_hiding_def sens_attrs_hiding_advantage_def)
+qed
 
-definition "perfect_hiding \<A> \<longleftrightarrow> (\<forall> query. valid_query query \<longrightarrow> hiding_advantage query \<A> = 0)" 
+definition token_hiding_game :: "('attrs, 'sens_atrrs, 'result) query \<Rightarrow> ('token, 'state,  'auth_token) hiding_adversary \<Rightarrow> bool spmf"
+  where 
+    "token_hiding_game query \<A> = do {
+      let (\<A>1, \<A>2) = \<A>;
+      ((token0, token1), \<sigma>) \<leftarrow> \<A>1;
+      _ :: unit \<leftarrow> assert_spmf (valid_token token0 \<and> valid_token token1);
+      b \<leftarrow> coin_spmf;
+      auth_token \<leftarrow> auth (if b then token1 else token0) query;
+      b' \<leftarrow> \<A>2 \<sigma> auth_token;  
+      return_spmf (b = b')}"
 
-definition soundness_game :: "'attrs \<Rightarrow> 'attrs query \<Rightarrow> 'token soundness_adversary \<Rightarrow> bool spmf"
-  where "soundness_game attrs query \<A> = do {
-        (token1, enc_user_record) \<leftarrow> reg attrs;
-        token2 \<leftarrow> \<A> token1;
-        _ :: unit \<leftarrow> assert_spmf (valid_token token2);
-        auth_token1 \<leftarrow> auth token1 query;
-        auth_token2 \<leftarrow> auth token2 query;
-        b :: bool \<leftarrow> ver auth_token1;
-        b' \<leftarrow> ver auth_token2;
-        return_spmf (b \<noteq> b')}"
+definition "token_hiding_advantage query \<A> = (\<bar>spmf (token_hiding_game query \<A>) True - 1/2\<bar>)"
 
-definition "soundness_advantage attrs query \<A> = \<bar>spmf (soundness_game attrs query \<A>) True\<bar>"
+definition "perfect_hiding \<A> \<longleftrightarrow> (\<forall> query. valid_query query \<longrightarrow> token_hiding_advantage query \<A> = 0)" 
 
-definition "perfect_soundness \<A> \<longleftrightarrow> (\<forall> attrs query. valid_attrs attrs \<longrightarrow> valid_query query \<longrightarrow> soundness_advantage attrs query \<A> = 0)"
+definition user_binding_game :: "'user \<Rightarrow> ('attrs, 'sens_atrrs, 'result) query \<Rightarrow> 'token soundness_adversary \<Rightarrow> bool spmf"
+  where 
+    "user_binding_game user query \<A> = do {
+      (token1, enc_user_record) \<leftarrow> reg user;
+      token2 \<leftarrow> \<A> token1;
+      _ :: unit \<leftarrow> assert_spmf (valid_token token2);
+      auth_token1 \<leftarrow> auth token1 query;
+      auth_token2 \<leftarrow> auth token2 query;
+      b :: 'result \<leftarrow> ver auth_token1;
+      b' \<leftarrow> ver auth_token2;
+      return_spmf (b \<noteq> b')}"
 
+definition "user_binding_advantage user query \<A> = \<bar>spmf (user_binding_game user query \<A>) True\<bar>"
+
+definition "perfect_soundness \<A> \<longleftrightarrow> (\<forall> user query. valid_user user \<longrightarrow> valid_query query \<longrightarrow> user_binding_advantage user query \<A> = 0)"
+
+end
+
+locale identity_ind_cpa_base = enc: ind_cpa key_gen encrypt decrypt valid_plains 
+  for key_gen :: "('pk \<times> 'sk) spmf"
+    and encrypt :: "'pk \<Rightarrow> 'sens_atrrs set \<Rightarrow> 'enc_attrs spmf"
+    and decrypt :: "'sk \<Rightarrow> 'enc_attrs \<Rightarrow> 'sens_atrrs set option"
+    and valid_plains :: "'sens_atrrs set \<Rightarrow> 'sens_atrrs set \<Rightarrow> bool"
+begin
+
+definition reg_enc_sens_attrs :: "'sens_atrrs set \<Rightarrow> 'enc_attrs spmf"
+  where 
+    "reg_enc_sens_attrs sens_attrs = do {
+      (pk,sk) \<leftarrow> key_gen;
+      encrypt pk sens_attrs}"   
+
+end 
+
+locale id_ind_cpa = identity_ind_cpa_base + 
+  id_sys: identity_system reg_enc_sens_attrs reg_govt_shares reg_govt_token auth ver valid_user valid_attrs valid_token valid_query user_set attrs_set users_attr_creation
+  for reg_govt_shares reg_govt_token auth ver valid_user valid_attrs valid_token valid_query user_set attrs_set users_attr_creation
+  + 
+  assumes users_are_valid: "user \<in> user_set \<longrightarrow> valid_user user"
+    and atrrs_are_valid: "attrs \<in> attrs_set \<longrightarrow> valid_attrs attrs"
+    and user_set_not_empty: "user_set \<noteq> {}"
+    and attrs_set_not_empty: "attrs_set \<noteq> {}"
+    and bij_betw_users_attrs: "bij_betw users_attr_creation user_set attrs_set"
+    and valid_user_valid_plains: "\<forall> u0 u1. valid_user u0 \<and> valid_user u1  \<longleftrightarrow> valid_plains (snd (users_attr_creation u0)) (snd (users_attr_creation u1))"
+begin
+
+
+definition sens_hiding_adversary1 :: "(('m \<times> 'm) \<times> 'n) spmf \<Rightarrow> 'a \<Rightarrow> (('c set \<times> 'c set) \<times> 'n) spmf"
+  where "sens_hiding_adversary1 \<A>1 pk = do {
+    ((u0,u1), \<sigma>) \<leftarrow> \<A>1;
+    _ :: unit \<leftarrow> assert_spmf (valid_user u0 \<and> valid_user u1);
+    let sens_set0 = snd (users_attr_creation u0);
+    let sens_set1 = snd (users_attr_creation u1);
+    return_spmf ((sens_set0, sens_set1), \<sigma>)}"
+
+definition sens_hiding_adversary2 :: "('n \<Rightarrow> 'd \<Rightarrow> bool spmf) \<Rightarrow> 'd \<Rightarrow> 'n \<Rightarrow> bool spmf"
+  where "sens_hiding_adversary2 \<A>2 enc \<sigma> = \<A>2 \<sigma> enc"
+
+fun sens_hiding_adversary:: "(('m \<times> 'm) \<times> 'n) spmf \<times> ('n \<Rightarrow> 'd \<Rightarrow> bool spmf) \<Rightarrow> ('a \<Rightarrow> (('c set \<times> 'c set) \<times> 'n) spmf) \<times> ('d \<Rightarrow> 'n \<Rightarrow> bool spmf)"
+  where "sens_hiding_adversary (\<A>1, \<A>2) = (sens_hiding_adversary1 \<A>1, sens_hiding_adversary2 \<A>2)"
+
+lemma if_cases_sens_hiding_attrs:
+  shows "(if b then fst (fst ((snd (users_attr_creation (fst (fst y))), snd (users_attr_creation (snd (fst y)))), snd y))
+             else snd (fst ((snd (users_attr_creation (fst (fst y))), snd (users_attr_creation (snd (fst y)))), snd y))) =
+                 snd (users_attr_creation (if b then fst (fst y) else snd (fst y)))"
+  by(cases b; auto)
+
+lemma sens_attrs_hiding_reduce_to_ind_cpa:
+  shows "id_sys.sens_attrs_hiding_advantage \<A> = enc.advantage (sens_hiding_adversary \<A>)"
+  including monad_normalisation
+proof-
+  note [simp] = split_def Let_def
+  obtain \<A>1 and \<A>2 where \<A> [simp]: "\<A> = (\<A>1, \<A>2)" by(cases \<A>)
+  have "id_sys.sens_attrs_hiding_advantage (\<A>1, \<A>2) = enc.advantage (sens_hiding_adversary1 \<A>1, sens_hiding_adversary2 \<A>2)"
+  proof-
+    have "TRY coin_spmf \<bind>
+           (\<lambda>b. key_gen \<bind>
+                 (\<lambda>y. \<A>1 \<bind>
+                       (\<lambda>p. encrypt (fst y) (snd (users_attr_creation (if b then fst (fst p) else snd (fst p)))) \<bind>
+                             (\<lambda>enc_attrs_b.
+                                 \<A>2 (snd p) enc_attrs_b \<bind> (\<lambda>b'. assert_spmf (valid_user (fst (fst p)) \<and> valid_user (snd (fst p))) 
+                                     \<bind> (\<lambda>_ :: unit. return_spmf (b' = b))))))) ELSE coin_spmf = 
+          TRY coin_spmf \<bind>
+                     (\<lambda>b. key_gen \<bind>
+                           (\<lambda>p. \<A>1 \<bind>
+                                 (\<lambda>y. encrypt (fst p) (snd (users_attr_creation (if b then fst (fst y) else snd (fst y)))) \<bind>
+                                       (\<lambda>cipher.
+                                           \<A>2 (snd y) cipher \<bind>
+                                           (\<lambda>b'. assert_spmf (valid_user (fst (fst y)) \<and> valid_user (snd (fst y))) \<bind>
+                                                  (\<lambda>ya :: unit. assert_spmf (valid_plains (snd (users_attr_creation (fst (fst y)))) (snd (users_attr_creation (snd (fst y))))) \<bind>
+                                                         (\<lambda>_ :: unit. return_spmf (b = b')))))))) ELSE coin_spmf"
+      apply(intro try_spmf_cong bind_spmf_cong[OF refl]; clarsimp?)+ using valid_user_valid_plains by force
+    thus ?thesis
+      unfolding id_sys.sens_attrs_hiding_advantage_def enc.advantage_def id_sys.sens_attrs_hiding_game_def 
+                enc.ind_cpa_def reg_enc_sens_attrs_def sens_hiding_adversary1_def sens_hiding_adversary2_def
+      by(auto simp add: if_cases_sens_hiding_attrs) 
+  qed
+  then show ?thesis by auto
+qed
+
+lemma perfect_sens_attrs_hiding:
+  "id_sys.perfect_sens_attrs_hiding \<A>" if "enc.advantage (sens_hiding_adversary \<A>) = 0"
+  unfolding id_sys.perfect_sens_attrs_hiding_def
+  by (simp add: sens_attrs_hiding_reduce_to_ind_cpa that)
+ 
 end
